Stack interpreter improved (#69)
* Update extraction/README.md

after a fix for the Liquidity dependency issue

* Improved the stack interpreter example: handling conditionals, more operations and example programs.

* Extraction-friendly names

extraction/examples/StackInterpreter.v
@@ -28,12 +28,15 @@ Definition action := ActionBody.
 
 Module Interpreter.
 
-  Inductive op : Set := Add | And | Equal.
+  Inductive op : Set :=  Add | Sub | Mult | Lt | Le | Equal.
 
   Inductive instruction :=
   | IPushZ : Z -> instruction
   | IPushB : bool -> instruction
-  | IObs : string -> Z -> instruction
+  | IObs : string * Z -> instruction
+  | IIf : instruction
+  | IElse : instruction
+  | IEndIf : instruction
   | IOp : op -> instruction.
 
   Inductive value : Set := BVal : bool -> value | ZVal : Z -> value.
@@ -44,45 +47,90 @@ Module Interpreter.
   Definition storage := list value.
 
   Definition init (ctx : SimpleCallCtx) (setup : unit) : option storage :=
-    let ctx' := ctx in (* prevents optimisations from removing unused [ctx]  *)
+    let ctx0 := ctx in (* prevents optimisations from removing unused [ctx]  *)
     Some [].
 
   Definition params := list instruction * ext_map.
 
-  Definition obs0 s := IObs s 0.
+  Definition obs0 s := IObs (s, 0%Z).
 
-  Fixpoint interp (ext : ext_map) (insts : list instruction) (s : list value) :=
+  Definition head_true_or_empty (l : list bool ) :=
+    match l with
+    | [] | true :: _ => true
+    | _ => false
+    end.
+
+  Open Scope Z.
+  Definition continue (i : Z) := (i =? 0)%Z.
+  Definition one := 1%Z.
+  Definition bool_to_cond (b : bool) : Z :=
+    if b then 0 else one.
+  Definition flip (i : Z) : Z :=
+    if (i =? 0) then one else if (i =? one) then 0 else i.
+  Definition reset_decrement (i : Z) : Z :=
+    if (i <=? one) then 0 else i-one.
+
+  Fixpoint interp (ext : ext_map) (insts : list instruction) (s : list value) (cond : Z) :=
     match insts with
     | [] => Some s
-    | hd :: inst' =>
-      match hd with
-      | IPushZ i => interp ext inst' (ZVal i :: s)
-      | IPushB b => interp ext inst' (BVal b :: s)
-      | IObs l i => match lookup (l,i) ext with
-                   | Some v => interp ext inst' (v :: s)
-                   | None => None
-                   end
-      | IOp op => match op with
-                   | Add => match s with
-                            | ZVal i :: ZVal j :: s' => interp ext inst' (ZVal (i+j) :: s')%Z
-                            | _ => None
+    | hd :: inst0 =>
+        match hd with
+        | IPushZ i => if continue cond then
+                       interp ext inst0 (ZVal i :: s) cond
+                     else interp ext inst0 s cond
+        | IPushB b => if continue cond then
+                       interp ext inst0 (BVal b :: s) cond
+                     else interp ext inst0 s cond
+        | IIf => if (cond =? 0) then
+                  match s with
+                  | BVal b :: s0 => interp ext inst0 s0 (bool_to_cond b)
+                  | _ => None
+                  end else interp ext inst0 s (one + cond)%Z
+        | IElse => interp ext inst0 s (flip cond)
+        | IEndIf => interp ext inst0 s (reset_decrement cond)
+        | IObs p =>
+          if continue cond then
+            match lookup p ext with
+            | Some v => interp ext inst0 (v :: s) cond
+            | None => None
+            end
+          else interp ext inst0 s cond
+        | IOp op =>
+          if continue cond then
+            match op with
+            | Add => match s with
+                    | ZVal i :: ZVal j :: s0 => interp ext inst0 (ZVal (i+j) :: s0)%Z cond
+                    | _ => None
+                    end
+            | Sub => match s with
+                      | ZVal i :: ZVal j :: s0 => interp ext inst0 (ZVal (i-j) :: s0)%Z cond
+                      | _ => None
+                      end
+            | Mult => match s with
+                     | ZVal i :: ZVal j :: s0 => interp ext inst0 (ZVal (i*j) :: s0)%Z cond
+                     | _ => None
                             end
-                   | And => match s with
-                            | BVal i :: BVal j :: s' => interp ext inst' (BVal (i && j) :: s')%Z
-                            | _ => None
-                           end
-                   | Equal => match s with
-                            | ZVal i :: ZVal j :: s' => interp ext inst' (BVal (i =? j) :: s')%Z
-                            | _ => None
-                             end
-                 end
-      end
-    end.
+            | Le => match s with
+                   | ZVal i :: ZVal j :: s0 => interp ext inst0 (BVal (i<=?j) :: s0)%Z cond
+                   | _ => None
+                   end
+            | Lt => match s with
+                   | ZVal i :: ZVal j :: s0 => interp ext inst0 (BVal (i<?j) :: s0)%Z cond
+                   | _ => None
+                   end
+            | Equal => match s with
+                      | ZVal i :: ZVal j :: s0 => interp ext inst0 (BVal (i =? j) :: s0)%Z cond
+                      | _ => None
+                     end
+            end
+          else interp ext inst0 s cond
+        end
+        end.
 
   Definition receive (p : params) (s : list value)
     : option (list action * storage) :=
-    let s' := s in (* prevents optimisations from removing unused [s]  *)
-    match interp p.2 p.1 [] with
+    let s0 := s in (* prevents optimisations from removing unused [s]  *)
+    match interp p.2 p.1 [] 0 with
     | Some v => Some ([],v)
     | None => None
     end.
@@ -91,13 +139,114 @@ End Interpreter.
 
 Import Interpreter.
 
-(** Input for the interpreter in Liquidity: *)
-(** ([IPushZ 0; IObs ("blah",0); IOp Add; IPushZ 1; IOp Equal], (Map [(("blah", 0), (ZVal 1))])) *)
+(** Input for the interpreter in Liquidity:
+    ([IPushZ 0; IObs ("blah",0); IOp Add; IPushZ 1; IOp Equal], (Map [(("blah", 0), (ZVal 1))])) *)
 Example test_interp :
   let env  := FMap.of_list [(("blah", 0%Z), (ZVal 1))] in
-  interp env [IPushZ 0; IObs "blah" 0; IOp Add; IPushZ 1; IOp Equal] [] =
+  interp env [IPushZ 0; IObs ("blah", 0); IOp Add; IPushZ 1; IOp Equal] [] 0 =
   Some [BVal true].
 Proof. reflexivity. Qed.
+
+(** Input for the interpreter in Liquidity:
+([IPushZ 1; IPushZ 1; IOp Equal; IIf; IPushZ 1;IElse; IPushZ (-1);IEndIf], (Map [])) *)
+Example test_interp_if_1 :
+  interp FMap.empty [IPushZ 1; IPushZ 1; IOp Equal; IIf; IPushZ 1;IElse; IPushZ (-1);IEndIf] [] 0
+  = Some [ZVal 1].
+Proof. reflexivity. Qed.
+
+Example test_interp_if_2 :
+  interp FMap.empty [IPushZ 1; IPushZ 0; IOp Equal; IIf; IPushZ 1;IElse; IPushZ (-1);IEndIf] [] 0
+  = Some [ZVal (-1)].
+Proof. reflexivity. Qed.
+
+Example test_interp_nested_if_1 :
+  interp FMap.empty [IPushZ 0;
+                    IPushZ 0;
+                    IOp Equal;
+                    IIf;
+                    IPushZ (-1)%Z;
+                    IPushZ (-1)%Z;
+                    IOp Equal;
+                    IIf;
+                    IPushZ 2;
+                    IElse;
+                    IPushZ (-2);
+                    IEndIf;
+                    IElse;
+                    IPushZ 0;
+                    IEndIf
+                    ] [] 0
+  = Some [ZVal 2].
+Proof. reflexivity. Qed.
+
+Example test_interp_nested_if_2 :
+  interp FMap.empty [IPushB false;
+                    IIf;
+                    IPushZ 1;
+                    IElse;
+                    IPushZ 0;
+                    IPushZ 0;
+                    IOp Equal;
+                    IIf;
+                    IPushZ (-1);
+                    IElse;
+                    IPushZ 0;
+                    IEndIf
+                    ] [] 0
+  = Some [ZVal (-1)].
+Proof. reflexivity. Qed.
+
+(*     let strike = 50.0
+        nominal = 1000.0
+        theobs = obs ("Carlsberg",0)
+    in scale (r nominal)
+             (transl maturity
+                    (iff (r strike !<! theobs)
+                          (scale (theobs - r strike)
+                                 (transfOne EUR "you" "me"))
+                         zero)) *)
+Definition call_option : list instruction :=
+  [IObs ("Maturity", 0);
+  IPushZ 90;
+  IOp Equal;
+  IIf;
+  IObs ("Carlsberg", 0);
+  IPushZ 50;
+  IOp Lt;
+  IIf;
+  IPushZ 50;
+  IObs ("Carlsberg", 0);
+  IOp Sub;
+  IPushZ 1000;
+  IOp Mult;
+  IElse;
+  IPushZ 0;
+  IEndIf;
+  IElse;
+  IPushZ 0;
+  IEndIf].
+
+(* ([IObs ("Maturity", 0);IPushZ 90;IOp Equal;IIf; IObs ("Carlsberg",0); IPushZ 50; IOp Lt; IIf; IPushZ 50; IObs ("Carlsberg", 0); IOp Sub; IPushZ 1000; IOp Mult; IElse; IPushZ 0; IEndIf; IElse; IPushZ 0; IEndIf], (Map [(("Carlsberg", 0), (ZVal 100));(("Maturity", 0), (ZVal 90))])) *)
+
+(* try-liquidty: estimated fee 0.054191 *)
+
+Example run_call_option_in_the_money :
+  let env := FMap.of_list [(("Carlsberg", 0%Z), (ZVal 100));(("Maturity", 0%Z), (ZVal 90))] in
+  interp env call_option [] 0
+  = Some [ZVal 50000].
+Proof. vm_compute. reflexivity. Qed.
+
+Example run_call_option_out_the_money :
+    let env := FMap.of_list [(("Carlsberg", 0%Z), (ZVal 30));(("Maturity", 0%Z), (ZVal 90))] in
+  interp env call_option [] 0
+  = Some [ZVal 0].
+Proof. reflexivity. Qed.
+
+(* A bigger test program for running in try-liquidity with arithmetic operations, lookups and some [Ifs] *)
+
+Definition blah := [IPushZ 100; IPushZ 200; IOp Add; IPushZ 200; IOp Add;IPushZ 100;IOp Add;IPushZ 100;IOp Add; IPushZ 200; IOp Add;IPushZ 100; IPushZ 200; IOp Add; IPushZ 200; IOp Add;IPushZ 100;IOp Add;IPushZ 100;IOp Add; IPushZ 200; IOp Add;IPushZ 100; IPushZ 200; IOp Add; IPushZ 200; IOp Add;IPushZ 100;IOp Add;IPushZ 100;IOp Add; IPushZ 200; IOp Add;IPushZ 100; IOp Add; IPushZ 200; IOp Add;IPushZ 100;IOp Add;IPushZ 100;IOp Add; IPushZ 200; IOp Add;IPushZ 100;IOp Mult; IPushZ 3000; IOp Sub; IPushZ 10; IOp Add; IPushZ 10; IOp Mult; IPushB true; IIf; IPushZ 10; IPushZ 10; IOp Equal; IIf; IPushZ 10; IPushZ 10; IOp Add; IPushZ 10; IOp Add;IElse; IPushB true; IEndIf;  IPushZ 10;IOp Add; IPushZ 10; IOp Add; IPushZ 10; IOp Add; IPushZ 10; IOp Mult; IObs ("blah", 0); IOp Add; IObs ("blah", 0); IOp Add; IObs ("blah", 0); IOp Add; IObs ("blah", 0); IOp Add; IObs ("blah", 0); IOp Add; IObs ("blah", 0); IOp Add; IObs ("blah", 0); IOp Add; IObs ("blah", 0); IOp Add; IObs ("blah", 0); IOp Add; IElse; IPushZ 0; IPushZ 0; IPushZ 0; IPushZ 0; IPushZ 0; IPushZ 0; IPushZ 0; IPushZ 0; IPushZ 0; IEndIf ].
+(* Just add the global environment (Map [(("blah", 0), (ZVal 0))])) *)
+Compute List.length blah.
 
 Definition print_finmap_type (prefix ty_key ty_val : string) :=
   parens false (ty_key ++ "," ++ prefix ++ ty_val) ++ " map".
@@ -118,11 +267,16 @@ Definition TT_remap : list (kername * string) :=
      ; remap <%% action %%> "operation"
      (* remapping operations *)
      ; remap <%% Z.add %%> "addInt"
+     ; remap <%% Z.mul %%> "mulInt"
+     ; remap <%% Z.sub %%> "subInt"
      ; remap <%% Z.eqb %%> "eqInt"
+     ; remap <%% Z.leb %%> "leInt"
+     ; remap <%% Z.ltb %%> "ltInt"
      ; remap <%% @lookup %%> "Map.find"
      ; remap <%% @fst %%> "fst"
      ; remap <%% @snd %%> "snd"
-       ; remap <%% andb %%> "andb" ].
+     ; remap <%% andb %%> "andb"
+     ; remap <%% one %%> "1"].
 
 Definition TT_rename : MyEnv.env string :=
      (* constructors *)
